Weidenbach_Book/IsaSAT_Lookup_Conflict.thy
@@ -105,22 +105,22 @@ qed
 context isasat_input_ops
 begin
 
-type_synonym (in -) conflict_rel = "nat \<times> bool option list"
+type_synonym (in -) lookup_clause_rel = "nat \<times> bool option list"
 
-definition conflict_rel :: "(conflict_rel \<times> nat literal multiset) set" where
-\<open>conflict_rel = {((n, xs), C). n = size C \<and> mset_as_position xs C \<and>
+definition lookup_clause_rel :: "(lookup_clause_rel \<times> nat literal multiset) set" where
+\<open>lookup_clause_rel = {((n, xs), C). n = size C \<and> mset_as_position xs C \<and>
    (\<forall>L\<in>atms_of \<L>\<^sub>a\<^sub>l\<^sub>l. L < length xs)}\<close>
 
-lemma conflict_rel_empty_iff: \<open>((n, xs), C) \<in> conflict_rel \<Longrightarrow> n = 0 \<longleftrightarrow> C = {#}\<close>
-  by (auto simp: conflict_rel_def)
+lemma lookup_clause_rel_empty_iff: \<open>((n, xs), C) \<in> lookup_clause_rel \<Longrightarrow> n = 0 \<longleftrightarrow> C = {#}\<close>
+  by (auto simp: lookup_clause_rel_def)
 
-lemma conflict_atm_le_length: \<open>((n, xs), C) \<in> conflict_rel \<Longrightarrow> L \<in> atms_of \<L>\<^sub>a\<^sub>l\<^sub>l \<Longrightarrow> L < length xs\<close>
-  by (auto simp: conflict_rel_def)
+lemma conflict_atm_le_length: \<open>((n, xs), C) \<in> lookup_clause_rel \<Longrightarrow> L \<in> atms_of \<L>\<^sub>a\<^sub>l\<^sub>l \<Longrightarrow> L < length xs\<close>
+  by (auto simp: lookup_clause_rel_def)
 
 
 lemma conflict_le_length:
   assumes
-    c_rel: \<open>((n, xs), C) \<in> conflict_rel\<close> and
+    c_rel: \<open>((n, xs), C) \<in> lookup_clause_rel\<close> and
     L_\<L>\<^sub>a\<^sub>l\<^sub>l: \<open>L \<in># \<L>\<^sub>a\<^sub>l\<^sub>l\<close>
   shows \<open>atm_of L < length xs\<close>
 proof -
@@ -128,27 +128,27 @@ proof -
     size: \<open>n = size C\<close> and
     mset_pos: \<open>mset_as_position xs C\<close> and
     atms_le: \<open>\<forall>L\<in>atms_of \<L>\<^sub>a\<^sub>l\<^sub>l. L < length xs\<close>
-    using c_rel unfolding conflict_rel_def by blast+
+    using c_rel unfolding lookup_clause_rel_def by blast+
   have \<open>atm_of L \<in> atms_of \<L>\<^sub>a\<^sub>l\<^sub>l\<close>
     using L_\<L>\<^sub>a\<^sub>l\<^sub>l by (simp add: atms_of_def)
   then show ?thesis
     using atms_le by blast
 qed
 
-lemma conflict_rel_atm_in_iff:
-  \<open>((n, xs), C) \<in> conflict_rel \<Longrightarrow> L \<in># \<L>\<^sub>a\<^sub>l\<^sub>l \<Longrightarrow> L \<in>#C \<longleftrightarrow> xs!(atm_of L) = Some (is_pos L)\<close>
+lemma lookup_clause_rel_atm_in_iff:
+  \<open>((n, xs), C) \<in> lookup_clause_rel \<Longrightarrow> L \<in># \<L>\<^sub>a\<^sub>l\<^sub>l \<Longrightarrow> L \<in>#C \<longleftrightarrow> xs!(atm_of L) = Some (is_pos L)\<close>
   by (rule mset_as_position_in_iff_nth)
-     (auto simp: conflict_rel_def atms_of_def)
+     (auto simp: lookup_clause_rel_def atms_of_def)
 
 lemma (in isasat_input_bounded)
-  assumes c: \<open>((n,xs), C) \<in> conflict_rel\<close>
+  assumes c: \<open>((n,xs), C) \<in> lookup_clause_rel\<close>
   shows
-    conflict_rel_not_tautolgy: \<open>\<not>tautology C\<close> and
-    conflict_rel_distinct_mset: \<open>distinct_mset C\<close> and
-    conflict_rel_size: \<open>literals_are_in_\<L>\<^sub>i\<^sub>n C \<Longrightarrow> size C \<le> 1 + uint_max div 2\<close>
+    lookup_clause_rel_not_tautolgy: \<open>\<not>tautology C\<close> and
+    lookup_clause_rel_distinct_mset: \<open>distinct_mset C\<close> and
+    lookup_clause_rel_size: \<open>literals_are_in_\<L>\<^sub>i\<^sub>n C \<Longrightarrow> size C \<le> 1 + uint_max div 2\<close>
 proof -
   have mset: \<open>mset_as_position xs C\<close> and \<open>n = size C\<close> and \<open>\<forall>L\<in>atms_of \<L>\<^sub>a\<^sub>l\<^sub>l. L < length xs\<close>
-    using c unfolding conflict_rel_def by fast+
+    using c unfolding lookup_clause_rel_def by fast+
   show \<open>\<not>tautology C\<close>
     using mset
     apply (induction rule: mset_as_position.induct)
@@ -161,82 +161,82 @@ proof -
     using simple_clss_size_upper_div2[of \<open>C\<close>] \<open>\<not>tautology C\<close> by auto
 qed
 
-type_synonym (in -) conflict_assn = "uint32 \<times> bool option array"
+type_synonym (in -) lookup_clause_assn = "uint32 \<times> bool option array"
 
-definition conflict_assn :: "nat clause \<Rightarrow> conflict_assn \<Rightarrow> assn" where
-\<open>conflict_assn = hr_comp (uint32_nat_assn *a array_assn (option_assn bool_assn)) conflict_rel\<close>
+definition lookup_clause_assn :: "nat clause \<Rightarrow> lookup_clause_assn \<Rightarrow> assn" where
+\<open>lookup_clause_assn = hr_comp (uint32_nat_assn *a array_assn (option_assn bool_assn)) lookup_clause_rel\<close>
 
-definition option_conflict_rel where
-\<open>option_conflict_rel = {((b,(n,xs)), C). b = (C = None) \<and>
-   (C = None \<longrightarrow> ((n,xs), {#}) \<in> conflict_rel) \<and>
-   (C \<noteq> None \<longrightarrow> ((n,xs), the C) \<in> conflict_rel)}
+definition option_lookup_clause_rel where
+\<open>option_lookup_clause_rel = {((b,(n,xs)), C). b = (C = None) \<and>
+   (C = None \<longrightarrow> ((n,xs), {#}) \<in> lookup_clause_rel) \<and>
+   (C \<noteq> None \<longrightarrow> ((n,xs), the C) \<in> lookup_clause_rel)}
    \<close>
 
-lemma option_conflict_rel_conflict_rel_iff:
-   \<open>((False, (n, xs)), Some C) \<in> option_conflict_rel \<longleftrightarrow>
-   ((n, xs), C) \<in> conflict_rel\<close>
-   unfolding option_conflict_rel_def by auto
+lemma option_lookup_clause_rel_lookup_clause_rel_iff:
+   \<open>((False, (n, xs)), Some C) \<in> option_lookup_clause_rel \<longleftrightarrow>
+   ((n, xs), C) \<in> lookup_clause_rel\<close>
+   unfolding option_lookup_clause_rel_def by auto
 
 
-type_synonym (in -) conflict_option_assn = "bool \<times> uint32 \<times> bool option array"
+type_synonym (in -) option_lookup_clause_assn = "bool \<times> uint32 \<times> bool option array"
 
-abbreviation (in -) conflict_rel_assn :: \<open>conflict_rel \<Rightarrow> conflict_assn \<Rightarrow> assn\<close> where
- \<open>conflict_rel_assn \<equiv> (uint32_nat_assn *a array_assn (option_assn bool_assn))\<close>
+abbreviation (in -) lookup_clause_rel_assn :: \<open>lookup_clause_rel \<Rightarrow> lookup_clause_assn \<Rightarrow> assn\<close> where
+ \<open>lookup_clause_rel_assn \<equiv> (uint32_nat_assn *a array_assn (option_assn bool_assn))\<close>
 
 type_synonym (in -) conflict_option_rel = \<open>bool \<times> nat \<times> bool option list\<close>
 
-abbreviation (in -)conflict_option_rel_assn :: \<open>conflict_option_rel \<Rightarrow> conflict_option_assn \<Rightarrow> assn\<close> where
- \<open>conflict_option_rel_assn \<equiv> (bool_assn *a conflict_rel_assn)\<close>
+abbreviation (in -)conflict_option_rel_assn :: \<open>conflict_option_rel \<Rightarrow> option_lookup_clause_assn \<Rightarrow> assn\<close> where
+ \<open>conflict_option_rel_assn \<equiv> (bool_assn *a lookup_clause_rel_assn)\<close>
 
-definition conflict_option_assn
-  :: \<open>nat clause option \<Rightarrow> conflict_option_assn \<Rightarrow> assn\<close>
+definition option_lookup_clause_assn
+  :: \<open>nat clause option \<Rightarrow> option_lookup_clause_assn \<Rightarrow> assn\<close>
 where
-  \<open>conflict_option_assn =
+  \<open>option_lookup_clause_assn =
      hr_comp (bool_assn *a uint32_nat_assn *a array_assn (option_assn bool_assn))
-       option_conflict_rel\<close>
+       option_lookup_clause_rel\<close>
 
-definition (in -) conflict_assn_is_None :: \<open>_ \<Rightarrow> bool\<close> where
-  \<open>conflict_assn_is_None = (\<lambda>(b, _, _). b)\<close>
+definition (in -) lookup_clause_assn_is_None :: \<open>_ \<Rightarrow> bool\<close> where
+  \<open>lookup_clause_assn_is_None = (\<lambda>(b, _, _). b)\<close>
 
-lemma conflict_assn_is_None_is_None: \<open>(RETURN o conflict_assn_is_None, RETURN o is_None) \<in>
-  option_conflict_rel \<rightarrow>\<^sub>f \<langle>bool_rel\<rangle>nres_rel\<close>
+lemma lookup_clause_assn_is_None_is_None: \<open>(RETURN o lookup_clause_assn_is_None, RETURN o is_None) \<in>
+  option_lookup_clause_rel \<rightarrow>\<^sub>f \<langle>bool_rel\<rangle>nres_rel\<close>
   by (intro nres_relI frefI)
-   (auto simp: option_conflict_rel_def conflict_assn_is_None_def split: option.splits)
+   (auto simp: option_lookup_clause_rel_def lookup_clause_assn_is_None_def split: option.splits)
 
-lemma conflict_assn_is_None_conflict_assn_is_None:
- \<open>(return o conflict_assn_is_None, RETURN o conflict_assn_is_None) \<in>
+lemma lookup_clause_assn_is_None_lookup_clause_assn_is_None:
+ \<open>(return o lookup_clause_assn_is_None, RETURN o lookup_clause_assn_is_None) \<in>
   conflict_option_rel_assn\<^sup>k \<rightarrow>\<^sub>a bool_assn\<close>
   by sepref_to_hoare
-   (sep_auto simp: conflict_assn_is_None_def)
+   (sep_auto simp: lookup_clause_assn_is_None_def)
 
-lemma conflict_assn_is_None_is_none_Code[sepref_fr_rules]:
-  \<open>(return \<circ> conflict_assn_is_None, RETURN \<circ> is_None) \<in> conflict_option_assn\<^sup>k \<rightarrow>\<^sub>a bool_assn\<close>
+lemma lookup_clause_assn_is_None_is_none_Code[sepref_fr_rules]:
+  \<open>(return \<circ> lookup_clause_assn_is_None, RETURN \<circ> is_None) \<in> option_lookup_clause_assn\<^sup>k \<rightarrow>\<^sub>a bool_assn\<close>
     (is \<open>_ \<in> [?pre]\<^sub>a ?im \<rightarrow> ?f\<close>)
-  using conflict_assn_is_None_conflict_assn_is_None[FCOMP conflict_assn_is_None_is_None,
-  unfolded conflict_option_assn_def[symmetric]] .
+  using lookup_clause_assn_is_None_lookup_clause_assn_is_None[FCOMP lookup_clause_assn_is_None_is_None,
+  unfolded option_lookup_clause_assn_def[symmetric]] .
 
-definition (in -) conflict_assn_is_empty :: \<open>_ \<Rightarrow> bool\<close> where
-  \<open>conflict_assn_is_empty = (\<lambda>(_, n, _). n = 0)\<close>
+definition (in -) lookup_clause_assn_is_empty :: \<open>_ \<Rightarrow> bool\<close> where
+  \<open>lookup_clause_assn_is_empty = (\<lambda>(_, n, _). n = 0)\<close>
 
-lemma conflict_assn_is_empty_is_empty:
-  \<open>(RETURN o conflict_assn_is_empty, RETURN o (\<lambda>D. Multiset.is_empty(the D))) \<in>
-  [\<lambda>D. D \<noteq> None]\<^sub>f option_conflict_rel \<rightarrow> \<langle>bool_rel\<rangle>nres_rel\<close>
+lemma lookup_clause_assn_is_empty_is_empty:
+  \<open>(RETURN o lookup_clause_assn_is_empty, RETURN o (\<lambda>D. Multiset.is_empty(the D))) \<in>
+  [\<lambda>D. D \<noteq> None]\<^sub>f option_lookup_clause_rel \<rightarrow> \<langle>bool_rel\<rangle>nres_rel\<close>
   by (intro nres_relI frefI)
-   (auto simp: option_conflict_rel_def conflict_assn_is_empty_def conflict_rel_def
+   (auto simp: option_lookup_clause_rel_def lookup_clause_assn_is_empty_def lookup_clause_rel_def
      Multiset.is_empty_def split: option.splits)
 
-lemma conflict_assn_is_empty_conflict_assn_is_empty:
- \<open>(return o conflict_assn_is_empty, RETURN o conflict_assn_is_empty) \<in>
+lemma lookup_clause_assn_is_empty_lookup_clause_assn_is_empty:
+ \<open>(return o lookup_clause_assn_is_empty, RETURN o lookup_clause_assn_is_empty) \<in>
   conflict_option_rel_assn\<^sup>k \<rightarrow>\<^sub>a bool_assn\<close>
   by sepref_to_hoare
-     (sep_auto simp: conflict_assn_is_empty_def uint32_nat_rel_def br_def nat_of_uint32_0_iff)
+     (sep_auto simp: lookup_clause_assn_is_empty_def uint32_nat_rel_def br_def nat_of_uint32_0_iff)
 
-lemma conflict_assn_is_empty_is_empty_code[sepref_fr_rules]:
-  \<open>(return \<circ> conflict_assn_is_empty, RETURN \<circ> the_is_empty) \<in>
-      [\<lambda>D. D \<noteq> None]\<^sub>a conflict_option_assn\<^sup>k \<rightarrow> bool_assn\<close>
-  using conflict_assn_is_empty_conflict_assn_is_empty[FCOMP conflict_assn_is_empty_is_empty,
-  unfolded conflict_option_assn_def[symmetric]] unfolding the_is_empty_def
-  conflict_option_assn_def[symmetric]
+lemma lookup_clause_assn_is_empty_is_empty_code[sepref_fr_rules]:
+  \<open>(return \<circ> lookup_clause_assn_is_empty, RETURN \<circ> the_is_empty) \<in>
+      [\<lambda>D. D \<noteq> None]\<^sub>a option_lookup_clause_assn\<^sup>k \<rightarrow> bool_assn\<close>
+  using lookup_clause_assn_is_empty_lookup_clause_assn_is_empty[FCOMP lookup_clause_assn_is_empty_is_empty,
+  unfolded option_lookup_clause_assn_def[symmetric]] unfolding the_is_empty_def
+  option_lookup_clause_assn_def[symmetric]
   by simp
 
 definition size_lookup_conflict :: \<open>_ \<Rightarrow> nat\<close> where
@@ -247,7 +247,7 @@ definition size_conflict_wl_heur :: \<open>_ \<Rightarrow> nat\<close> where
 
 lemma size_lookup_conflict[sepref_fr_rules]:
    \<open>(return o (\<lambda>((_, n, _), _). n), RETURN o size_lookup_conflict) \<in>
-   (((bool_assn *a conflict_rel_assn) *a
+   (((bool_assn *a lookup_clause_rel_assn) *a
          option_assn (unat_lit_assn *a uint32_nat_assn)))\<^sup>k \<rightarrow>\<^sub>a uint32_nat_assn\<close>
   unfolding size_lookup_conflict_def
   apply sep_auto
@@ -313,7 +313,7 @@ definition (in -) is_in_lookup_conflict where
 sepref_thm is_in_conflict_code
   is \<open>uncurry (RETURN oo is_in_lookup_conflict)\<close>
   :: \<open>[\<lambda>((n, xs), L). atm_of L < length xs]\<^sub>a
-       conflict_rel_assn\<^sup>k *\<^sub>a unat_lit_assn\<^sup>k \<rightarrow> bool_assn\<close>
+       lookup_clause_rel_assn\<^sup>k *\<^sub>a unat_lit_assn\<^sup>k \<rightarrow> bool_assn\<close>
   supply length_rll_def[simp] nth_rll_def[simp] uint_max_def[simp] uint32_nat_assn_one[sepref_fr_rules]
   image_image[simp]
   unfolding is_in_lookup_conflict_def
@@ -332,17 +332,17 @@ definition conflict_merge :: \<open>(nat, nat) ann_lits \<Rightarrow> nat clause
   (nat clause option \<times> nat) nres\<close> where
 \<open>conflict_merge M N i _ _ = RES {(Some (mset (N!i)), card_max_lvl M (mset (N!i)))}\<close>
 
-definition add_to_lookup_conflict :: \<open>nat literal \<Rightarrow> conflict_rel \<Rightarrow> conflict_rel\<close> where
+definition add_to_lookup_conflict :: \<open>nat literal \<Rightarrow> lookup_clause_rel \<Rightarrow> lookup_clause_rel\<close> where
   \<open>add_to_lookup_conflict = (\<lambda>L (n, xs). (if xs ! atm_of L = None then n + 1 else n,
       xs[atm_of L := Some (is_pos L)]))\<close>
 
 
-definition lookup_conflict_merge'_step :: \<open>(nat, nat) ann_lits \<Rightarrow> nat \<Rightarrow> nat \<Rightarrow> conflict_rel \<Rightarrow> nat clause_l \<Rightarrow>
+definition lookup_conflict_merge'_step :: \<open>(nat, nat) ann_lits \<Rightarrow> nat \<Rightarrow> nat \<Rightarrow> lookup_clause_rel \<Rightarrow> nat clause_l \<Rightarrow>
       nat clause \<Rightarrow> bool\<close> where
   \<open>lookup_conflict_merge'_step M i clvls zs D C = (
       let D' = mset (take i D);
           E = remdups_mset (D' + (C - D' - image_mset uminus D')) in
-      ((False, zs), Some E) \<in> option_conflict_rel \<and>
+      ((False, zs), Some E) \<in> option_lookup_clause_rel \<and>
       literals_are_in_\<L>\<^sub>i\<^sub>n E \<and> clvls = card_max_lvl M E)\<close>
 
 lemma (in isasat_input_ops)mset_as_position_remove:
@@ -373,16 +373,16 @@ next
   qed
 qed
 
-lemma option_conflict_rel_update_None:
-  assumes  \<open>((False, (n, xs)), Some D) \<in> option_conflict_rel\<close> and L_xs : \<open>L < length xs\<close>
+lemma option_lookup_clause_rel_update_None:
+  assumes  \<open>((False, (n, xs)), Some D) \<in> option_lookup_clause_rel\<close> and L_xs : \<open>L < length xs\<close>
   shows \<open>((False, (if xs!L = None then n else n - 1, xs[L := None])),
-      Some (D - {# Pos L, Neg L #})) \<in> option_conflict_rel\<close>
+      Some (D - {# Pos L, Neg L #})) \<in> option_lookup_clause_rel\<close>
 proof -
   have [simp]: "L \<notin># A \<Longrightarrow> A - add_mset L' (add_mset L B) = A - add_mset L' B"
     for A B :: \<open>'a multiset\<close> and L L'
     by (metis add_mset_commute minus_notin_trivial)
   have "n = size D" and map: "mset_as_position xs D"
-    using assms by (auto simp: option_conflict_rel_def conflict_rel_def)
+    using assms by (auto simp: option_lookup_clause_rel_def lookup_clause_rel_def)
   have xs_None_iff: "xs ! L = None \<longleftrightarrow> Pos L \<notin># D \<and> Neg L \<notin># D"
     using map L_xs mset_as_position_in_iff_nth[of xs D "Pos L"] mset_as_position_in_iff_nth[of xs D "Neg L"]
     by (cases \<open>xs ! L\<close>) auto
@@ -397,20 +397,20 @@ proof -
 
   show ?thesis
     using assms mset_as_position_remove[of xs D L]
-    by (auto simp: option_conflict_rel_def conflict_rel_def 1 2 3 size_remove1_mset_If minus_notin_trivial
+    by (auto simp: option_lookup_clause_rel_def lookup_clause_rel_def 1 2 3 size_remove1_mset_If minus_notin_trivial
         mset_as_position_remove)
 qed
 
 
-lemma add_to_lookup_conflict_conflict_rel:
-  assumes confl: \<open>((n, xs), C) \<in> conflict_rel\<close> and uL_C: \<open>-L \<notin># C\<close> and L_\<L>\<^sub>a\<^sub>l\<^sub>l: \<open>L \<in># \<L>\<^sub>a\<^sub>l\<^sub>l\<close>
-  shows \<open>(add_to_lookup_conflict L (n, xs), {#L#} \<union># C) \<in> conflict_rel\<close>
+lemma add_to_lookup_conflict_lookup_clause_rel:
+  assumes confl: \<open>((n, xs), C) \<in> lookup_clause_rel\<close> and uL_C: \<open>-L \<notin># C\<close> and L_\<L>\<^sub>a\<^sub>l\<^sub>l: \<open>L \<in># \<L>\<^sub>a\<^sub>l\<^sub>l\<close>
+  shows \<open>(add_to_lookup_conflict L (n, xs), {#L#} \<union># C) \<in> lookup_clause_rel\<close>
 proof -
   have
     n: \<open>n = size C\<close> and
     mset: \<open>mset_as_position xs C\<close> and
     atm: \<open>\<forall>L\<in>atms_of \<L>\<^sub>a\<^sub>l\<^sub>l. L < length xs\<close>
-    using confl unfolding conflict_rel_def by blast+
+    using confl unfolding lookup_clause_rel_def by blast+
   have \<open>distinct_mset C\<close>
     using mset by (blast dest: mset_as_position_distinct_mset)
   have atm_L_xs: \<open>atm_of L < length xs\<close>
@@ -424,7 +424,7 @@ proof -
       using True by (simp add: subset_mset.sup.absorb2)
     ultimately show ?thesis
       using n mset atm True
-      by (auto simp: conflict_rel_def add_to_lookup_conflict_def xs[symmetric])
+      by (auto simp: lookup_clause_rel_def add_to_lookup_conflict_def xs[symmetric])
   next
     case False
     with mset have \<open>xs ! atm_of L = None\<close>
@@ -433,7 +433,7 @@ proof -
       by (cases L; cases \<open>xs ! atm_of L\<close>) auto
     then show ?thesis
       using n mset atm False atm_L_xs uL_C
-      by (auto simp: conflict_rel_def add_to_lookup_conflict_def
+      by (auto simp: lookup_clause_rel_def add_to_lookup_conflict_def
           intro!: mset_as_position.intros)
   qed
 qed
@@ -488,13 +488,13 @@ lemmas lookup_conflict_merge_aa_hnr[sepref_fr_rules] =
 
 lemma lookup_conflict_merge'_spec:
   assumes
-      o: \<open>((b, n, xs), Some C) \<in> option_conflict_rel\<close> and
+      o: \<open>((b, n, xs), Some C) \<in> option_lookup_clause_rel\<close> and
       dist: \<open>distinct D\<close> and
       lits: \<open>literals_are_in_\<L>\<^sub>i\<^sub>n (mset D)\<close> and
       tauto: \<open>\<not>tautology (mset D)\<close> and
       \<open>literals_are_in_\<L>\<^sub>i\<^sub>n C\<close> and
       \<open>clvls = card_max_lvl M C\<close>
-  shows \<open>lookup_conflict_merge M D (b, n, xs) clvls \<le> \<Down> (option_conflict_rel \<times>\<^sub>r Id)
+  shows \<open>lookup_conflict_merge M D (b, n, xs) clvls \<le> \<Down> (option_lookup_clause_rel \<times>\<^sub>r Id)
              (RES {(Some (mset D \<union># (C - mset D - uminus `# mset D)),
               card_max_lvl M (mset D \<union># (C - mset D - uminus `# mset D)))})\<close>
 proof -
@@ -508,39 +508,39 @@ proof -
      atms_le_xs: \<open>\<forall>L\<in>atms_of \<L>\<^sub>a\<^sub>l\<^sub>l. L < length xs\<close> and
      map: \<open>mset_as_position xs C\<close>
     using assms simple_clss_size_upper_div2[of C] mset_as_position_distinct_mset[of xs C]
-      conflict_rel_not_tautolgy[of n xs C]
-    unfolding option_conflict_rel_def conflict_rel_def
+      lookup_clause_rel_not_tautolgy[of n xs C]
+    unfolding option_lookup_clause_rel_def lookup_clause_rel_def
     by (auto simp: uint_max_def)
   then have clvls_uint_max: \<open>clvls \<le> 1 + uint_max div 2\<close>
     using size_filter_mset_lesseq[of \<open>\<lambda>L. get_level M L = count_decided M\<close> C]
     unfolding uint_max_def card_max_lvl_def by linarith
-  have [intro]: \<open>((b, a, ba), Some C) \<in> option_conflict_rel \<Longrightarrow> literals_are_in_\<L>\<^sub>i\<^sub>n C \<Longrightarrow>
+  have [intro]: \<open>((b, a, ba), Some C) \<in> option_lookup_clause_rel \<Longrightarrow> literals_are_in_\<L>\<^sub>i\<^sub>n C \<Longrightarrow>
         Suc (Suc a) \<le> uint_max\<close> for b a ba C
-    using conflict_rel_size[of a ba C] by (auto simp: option_conflict_rel_def
-        conflict_rel_def uint_max_def)
+    using lookup_clause_rel_size[of a ba C] by (auto simp: option_lookup_clause_rel_def
+        lookup_clause_rel_def uint_max_def)
   have [simp]: \<open>remdups_mset C = C\<close>
-    using o mset_as_position_distinct_mset[of xs C] by (auto simp: option_conflict_rel_def conflict_rel_def
+    using o mset_as_position_distinct_mset[of xs C] by (auto simp: option_lookup_clause_rel_def lookup_clause_rel_def
         distinct_mset_remdups_mset_id)
   have \<open>\<not>tautology C\<close>
-    using mset_as_position_tautology o by (auto simp: option_conflict_rel_def
-        conflict_rel_def)
+    using mset_as_position_tautology o by (auto simp: option_lookup_clause_rel_def
+        lookup_clause_rel_def)
   have \<open>distinct_mset C\<close>
     using mset_as_position_distinct_mset[of _ C] o
-    unfolding option_conflict_rel_def conflict_rel_def by auto
+    unfolding option_lookup_clause_rel_def lookup_clause_rel_def by auto
   let ?C' = \<open>\<lambda>a. mset (take a D) + (C - (mset (take a D) + uminus `# mset (take a D)))\<close>
   have tauto_C': \<open>\<not> tautology (?C' a)\<close> for a
     using tauto tauto_C dist dist_C unfolding tautology_decomp'
     by (auto dest: in_set_takeD in_diffD simp: distinct_mset_in_diff in_image_uminus_uminus)
 
   define I where
-     \<open>I xs = (\<lambda>(i, clvls, zs :: conflict_rel).
+     \<open>I xs = (\<lambda>(i, clvls, zs :: lookup_clause_rel).
                      i \<le> length D \<and>
                      length (snd zs) =
                      length (snd xs) \<and>
                      Suc i \<le> uint_max \<and>
                      Suc (fst zs) \<le> uint_max \<and>
                      Suc clvls \<le> uint_max)\<close>
-   for xs :: conflict_rel
+   for xs :: lookup_clause_rel
   define I' where \<open>I' = (\<lambda>(i, clvls, zs). lookup_conflict_merge'_step M i clvls zs D C)\<close>
   have
     if_True_I: \<open>I x2 (Suc a, aa + 1, add_to_lookup_conflict (D ! a) baa)\<close> (is ?I) and
@@ -563,7 +563,7 @@ proof -
     obtain ab b where baa[simp]: \<open>baa = (ab, b)\<close> by (cases baa)
 
     have aa: \<open>aa = card_max_lvl M (remdups_mset (?C' a))\<close> and
-      ocr: \<open>((False, ab, b), Some (remdups_mset (?C' a))) \<in> option_conflict_rel\<close> and
+      ocr: \<open>((False, ab, b), Some (remdups_mset (?C' a))) \<in> option_lookup_clause_rel\<close> and
       lits: \<open>literals_are_in_\<L>\<^sub>i\<^sub>n (remdups_mset (?C' a))\<close>
       using I'
       unfolding I'_def lookup_conflict_merge'_step_def Let_def
@@ -572,8 +572,8 @@ proof -
       ab: \<open>ab = size (remdups_mset (?C' a))\<close> and
       map: \<open>mset_as_position b (remdups_mset (?C' a))\<close> and
       \<open>\<forall>L\<in>atms_of \<L>\<^sub>a\<^sub>l\<^sub>l. L < length b\<close> and
-      cr: \<open>((ab, b), remdups_mset (?C' a)) \<in> conflict_rel\<close>
-      using ocr unfolding option_conflict_rel_def conflict_rel_def
+      cr: \<open>((ab, b), remdups_mset (?C' a)) \<in> lookup_clause_rel\<close>
+      using ocr unfolding option_lookup_clause_rel_def lookup_clause_rel_def
       by auto
 
     have \<open>size (card_max_lvl M (remdups_mset (?C' a))) \<le> size (remdups_mset (?C' a))\<close>
@@ -590,7 +590,7 @@ proof -
 
     have ab_upper: \<open>Suc (Suc ab) \<le> uint_max\<close>
       using simple_clss_size_upper_div2[of \<open>remdups_mset (?C' a)\<close>]
-      conflict_rel_not_tautolgy[OF cr] a_le_D lits mset_as_position_distinct_mset[OF map]
+      lookup_clause_rel_not_tautolgy[OF cr] a_le_D lits mset_as_position_distinct_mset[OF map]
       unfolding ab literals_are_in_\<L>\<^sub>i\<^sub>n_remdups uint_max_def by auto
     show ?I
       using le_D_le_upper a_le_D ab_upper
@@ -616,9 +616,9 @@ proof -
       by (auto simp: in_\<L>\<^sub>a\<^sub>l\<^sub>l_atm_of_in_atms_of_iff)
 
     have ocr: \<open>((False, add_to_lookup_conflict (D ! a) (ab, b)), Some (remdups_mset (?C' (Suc a))))
-        \<in> option_conflict_rel\<close>
+        \<in> option_lookup_clause_rel\<close>
       using ocr D_a_notin uD_a_notin
-      unfolding option_conflict_rel_def conflict_rel_def add_to_lookup_conflict_def
+      unfolding option_lookup_clause_rel_def lookup_clause_rel_def add_to_lookup_conflict_def
       by (auto dest: in_diffD simp: minus_notin_trivial
           intro!: mset_as_position.intros)
 
@@ -651,7 +651,7 @@ proof -
     obtain ab b where baa[simp]: \<open>baa = (ab, b)\<close> by (cases baa)
 
     have aa: \<open>aa = card_max_lvl M (remdups_mset (?C' a))\<close> and
-      ocr: \<open>((False, ab, b), Some (remdups_mset (?C' a))) \<in> option_conflict_rel\<close> and
+      ocr: \<open>((False, ab, b), Some (remdups_mset (?C' a))) \<in> option_lookup_clause_rel\<close> and
       lits: \<open>literals_are_in_\<L>\<^sub>i\<^sub>n (remdups_mset (?C' a))\<close>
       using I'
       unfolding I'_def lookup_conflict_merge'_step_def Let_def
@@ -660,8 +660,8 @@ proof -
       ab: \<open>ab = size (remdups_mset (?C' a))\<close> and
       map': \<open>mset_as_position b (remdups_mset (?C' a))\<close> and
       \<open>\<forall>L\<in>atms_of \<L>\<^sub>a\<^sub>l\<^sub>l. L < length b\<close> and
-      cr: \<open>((ab, b), remdups_mset (?C' a)) \<in> conflict_rel\<close>
-      using ocr unfolding option_conflict_rel_def conflict_rel_def
+      cr: \<open>((ab, b), remdups_mset (?C' a)) \<in> lookup_clause_rel\<close>
+      using ocr unfolding option_lookup_clause_rel_def lookup_clause_rel_def
       by auto
 
     have \<open>size (card_max_lvl M (remdups_mset (?C' a))) \<le> size (remdups_mset (?C' a))\<close>
@@ -678,7 +678,7 @@ proof -
 
     have ab_upper: \<open>Suc (Suc ab) \<le> uint_max\<close>
       using simple_clss_size_upper_div2[of \<open>remdups_mset (?C' a)\<close>]
-      conflict_rel_not_tautolgy[OF cr] a_le_D lits mset_as_position_distinct_mset[OF map']
+      lookup_clause_rel_not_tautolgy[OF cr] a_le_D lits mset_as_position_distinct_mset[OF map']
       unfolding ab literals_are_in_\<L>\<^sub>i\<^sub>n_remdups uint_max_def by auto
     show ?I
       using a_le_D ab_upper Suc_Suc_aa
@@ -711,7 +711,7 @@ proof -
        (SomeF) \<open>b ! atm_of (D ! a) = Some False\<close>
       by (cases \<open>b ! atm_of (D ! a)\<close>) auto
     then have ocr: \<open>((False, add_to_lookup_conflict (D ! a) (ab, b)), Some (remdups_mset (?C' (Suc a))))
-      \<in> option_conflict_rel\<close>
+      \<in> option_lookup_clause_rel\<close>
     proof cases
       case [simp]: None
       have [simp]: \<open>D ! a \<notin># C\<close> \<open>-D ! a \<notin># C\<close>
@@ -723,9 +723,9 @@ proof -
         using literals_are_in_\<L>\<^sub>i\<^sub>n_in_\<L>\<^sub>a\<^sub>l\<^sub>l[OF \<open>literals_are_in_\<L>\<^sub>i\<^sub>n (mset D)\<close> a_le_D] atms_le_xs
         by (auto simp: in_\<L>\<^sub>a\<^sub>l\<^sub>l_atm_of_in_atms_of_iff)
 
-      show ocr: \<open>((False, add_to_lookup_conflict (D ! a) (ab, b)), Some (remdups_mset (?C' (Suc a)))) \<in> option_conflict_rel\<close>
+      show ocr: \<open>((False, add_to_lookup_conflict (D ! a) (ab, b)), Some (remdups_mset (?C' (Suc a)))) \<in> option_lookup_clause_rel\<close>
         using ocr D_a_notin uD_a_notin
-        unfolding option_conflict_rel_def conflict_rel_def add_to_lookup_conflict_def
+        unfolding option_lookup_clause_rel_def lookup_clause_rel_def add_to_lookup_conflict_def
         by (auto dest: in_diffD simp: minus_notin_trivial
             intro!: mset_as_position.intros)
     next
@@ -777,7 +777,7 @@ proof -
         done
       show ?thesis
         using uDa_C SomeT dist_C  map'' atms_le_xs
-        unfolding option_conflict_rel_def conflict_rel_def add_to_lookup_conflict_def ab Da_def[symmetric] C'
+        unfolding option_lookup_clause_rel_def lookup_clause_rel_def add_to_lookup_conflict_def ab Da_def[symmetric] C'
         by (auto dest:  simp: distinct_mset_in_diff minus_notin_trivial
             intro: mset_as_position.intros)
     next
@@ -830,7 +830,7 @@ proof -
         done
       show ?thesis
         using uDa_C SomeF dist_C  map'' atms_le_xs
-        unfolding option_conflict_rel_def conflict_rel_def add_to_lookup_conflict_def ab Da_def[symmetric] C'
+        unfolding option_lookup_clause_rel_def lookup_clause_rel_def add_to_lookup_conflict_def ab Da_def[symmetric] C'
         by (auto dest:  simp: distinct_mset_in_diff minus_notin_trivial
             intro: mset_as_position.intros)
     qed
@@ -884,7 +884,7 @@ proof -
       subgoal by simp
       subgoal using map' mset_as_position_tautology by blast
       subgoal by simp
-      subgoal using ocr unfolding option_conflict_rel_def conflict_rel_def
+      subgoal using ocr unfolding option_lookup_clause_rel_def lookup_clause_rel_def
         by (auto dest!: mset_as_position_tautology)
       done }
     ultimately show ?I'
@@ -899,7 +899,7 @@ proof -
   have dist_CD: \<open>distinct_mset (C - mset D - uminus `# mset D)\<close>
     using \<open>distinct_mset C\<close> by auto
   have confl: \<open>lookup_conflict_merge M D (b, n, xs) clvls
-    \<le> \<Down> (option_conflict_rel \<times>\<^sub>r Id)
+    \<le> \<Down> (option_lookup_clause_rel \<times>\<^sub>r Id)
        (RES {(Some (mset D \<union># (C - mset D - uminus `# mset D)),
               card_max_lvl M (mset D \<union># (C - mset D - uminus `# mset D)))})\<close>
     unfolding lookup_conflict_merge_aa_def lookup_conflict_merge_def PR_CONST_def
@@ -909,20 +909,20 @@ proof -
     subgoal by auto
     subgoal using clvls_uint_max Suc_N_uint_max unfolding uint_max_def I_def by auto
     subgoal using assms
-      unfolding lookup_conflict_merge'_step_def Let_def option_conflict_rel_def I'_def
-      by (auto simp add: uint_max_def lookup_conflict_merge'_step_def option_conflict_rel_def)
+      unfolding lookup_conflict_merge'_step_def Let_def option_lookup_clause_rel_def I'_def
+      by (auto simp add: uint_max_def lookup_conflict_merge'_step_def option_lookup_clause_rel_def)
     subgoal by auto
     subgoal unfolding I_def by fast
     subgoal by (rule if_True_I)
     subgoal by (rule if_true_I')
     subgoal for b' n' s j zs
       using dist lits tauto
-      by (auto simp: option_conflict_rel_def take_Suc_conv_app_nth
+      by (auto simp: option_lookup_clause_rel_def take_Suc_conv_app_nth
           literals_are_in_\<L>\<^sub>i\<^sub>n_in_\<L>\<^sub>a\<^sub>l\<^sub>l)
     subgoal by (rule if_False_I)
     subgoal by (rule if_False_I')
     subgoal by auto
-    subgoal using assms by (auto simp: option_conflict_rel_def lookup_conflict_merge'_step_def Let_def
+    subgoal using assms by (auto simp: option_lookup_clause_rel_def lookup_conflict_merge'_step_def Let_def
           I_def I'_def)
     done
   have count_D: \<open>count (mset D) a = 1 \<or> count (mset D) a = 0\<close> for a
@@ -943,18 +943,18 @@ lemma lookup_conflict_merge_aa_set_conflict:
   \<open>(uncurry4 lookup_conflict_merge_aa, uncurry4 conflict_merge) \<in>
     [\<lambda>((((M, N), i), xs), clvls). i < length N \<and> xs = None \<and> distinct (N ! i) \<and>
        literals_are_in_\<L>\<^sub>i\<^sub>n (mset (N ! i)) \<and> \<not>tautology (mset (N ! i)) \<and> clvls = 0]\<^sub>f
-    \<langle>Id\<rangle>list_rel \<times>\<^sub>f \<langle>\<langle>Id\<rangle>list_rel\<rangle>list_rel \<times>\<^sub>f nat_rel \<times>\<^sub>f option_conflict_rel \<times>\<^sub>f nat_rel \<rightarrow>
-      \<langle>option_conflict_rel \<times>\<^sub>f nat_rel\<rangle>nres_rel\<close>
+    \<langle>Id\<rangle>list_rel \<times>\<^sub>f \<langle>\<langle>Id\<rangle>list_rel\<rangle>list_rel \<times>\<^sub>f nat_rel \<times>\<^sub>f option_lookup_clause_rel \<times>\<^sub>f nat_rel \<rightarrow>
+      \<langle>option_lookup_clause_rel \<times>\<^sub>f nat_rel\<rangle>nres_rel\<close>
 proof -
   have [simp]: \<open>\<not>tautology (mset C) \<Longrightarrow> j < length C \<Longrightarrow> -C ! j \<notin> set (take j C)\<close> for j C
     by (meson in_multiset_in_set in_set_takeD nth_mem_mset tautology_minus)
   have [simp]: \<open>distinct C \<Longrightarrow> j < length C \<Longrightarrow> C ! j \<notin> set (take j C)\<close> for j C
     by (simp add: index_nth_id index_take)
-  have H: \<open>lookup_conflict_merge_aa M N i (b, n, xs) clvls \<le> \<Down> (option_conflict_rel \<times>\<^sub>r nat_rel)
+  have H: \<open>lookup_conflict_merge_aa M N i (b, n, xs) clvls \<le> \<Down> (option_lookup_clause_rel \<times>\<^sub>r nat_rel)
       (conflict_merge M N i None clvls)\<close>
     if
       \<open>i < length N\<close> and
-      ocr: \<open>((b, n, xs), None) \<in> option_conflict_rel\<close> and
+      ocr: \<open>((b, n, xs), None) \<in> option_lookup_clause_rel\<close> and
      dist: \<open>distinct (N! i)\<close> and
      lits: \<open>literals_are_in_\<L>\<^sub>i\<^sub>n (mset (N ! i))\<close> and
      tauto: \<open>\<not>tautology (mset (N ! i))\<close> and
@@ -966,8 +966,8 @@ proof -
     have lookup_conflict_merge_normalise: \<open>lookup_conflict_merge M C (b, zs) = lookup_conflict_merge M C (False, zs)\<close>
       for M C zs
       unfolding lookup_conflict_merge_def by auto
-    have T: \<open>((False, n, xs), Some {#}) \<in> option_conflict_rel\<close>
-      using ocr unfolding option_conflict_rel_def by auto
+    have T: \<open>((False, n, xs), Some {#}) \<in> option_lookup_clause_rel\<close>
+      using ocr unfolding option_lookup_clause_rel_def by auto
     then show ?thesis unfolding lookup_conflict_merge_aa_def conflict_merge_def
       using lookup_conflict_merge'_spec[of False n xs \<open>{#}\<close> \<open>N!i\<close>] that dist
       by (auto simp: lookup_conflict_merge_normalise)
@@ -981,14 +981,14 @@ theorem lookup_conflict_merge_code_set_conflict[sepref_fr_rules]:
   \<open>(uncurry4 lookup_conflict_merge_code, uncurry4 conflict_merge) \<in>
   [\<lambda>((((M, N), i), xs), clvls). clvls = 0 \<and> i < length N \<and> xs = None \<and> distinct (N ! i) \<and>
     literals_are_in_\<L>\<^sub>i\<^sub>n (mset (N ! i)) \<and> \<not> tautology (mset (N ! i))]\<^sub>a
-  trail_assn\<^sup>k *\<^sub>a clauses_ll_assn\<^sup>k *\<^sub>a nat_assn\<^sup>k *\<^sub>a conflict_option_assn\<^sup>d *\<^sub>a uint32_nat_assn\<^sup>k \<rightarrow>
-    conflict_option_assn *a uint32_nat_assn\<close>
+  trail_assn\<^sup>k *\<^sub>a clauses_ll_assn\<^sup>k *\<^sub>a nat_assn\<^sup>k *\<^sub>a option_lookup_clause_assn\<^sup>d *\<^sub>a uint32_nat_assn\<^sup>k \<rightarrow>
+    option_lookup_clause_assn *a uint32_nat_assn\<close>
    (is \<open>?c \<in> [?pre]\<^sub>a ?im \<rightarrow> ?f\<close>)
 proof -
    have H: \<open>?c
   \<in> [comp_PRE
      (\<langle>Id\<rangle>list_rel \<times>\<^sub>f \<langle>\<langle>Id\<rangle>list_rel\<rangle>list_rel \<times>\<^sub>f nat_rel \<times>\<^sub>f
-      option_conflict_rel \<times>\<^sub>f
+      option_lookup_clause_rel \<times>\<^sub>f
       nat_rel)
      (\<lambda>((((M, N), i), xs), clvls).
          i < length N \<and>
@@ -1008,11 +1008,11 @@ proof -
                      uint32_nat_assn\<^sup>k)
                     (\<langle>Id\<rangle>list_rel \<times>\<^sub>f \<langle>\<langle>Id\<rangle>list_rel\<rangle>list_rel \<times>\<^sub>f
                      nat_rel \<times>\<^sub>f
-                     option_conflict_rel \<times>\<^sub>f
+                     option_lookup_clause_rel \<times>\<^sub>f
                      nat_rel) \<rightarrow> hr_comp
                                   (conflict_option_rel_assn *a
                                    uint32_nat_assn)
-                                  (option_conflict_rel \<times>\<^sub>f nat_rel)\<close>
+                                  (option_lookup_clause_rel \<times>\<^sub>f nat_rel)\<close>
    (is \<open>_ \<in> [?pre']\<^sub>a ?im' \<rightarrow> ?f'\<close>)
      using hfref_compI_PRE_aux[OF lookup_conflict_merge_code.refine[unfolded PR_CONST_def]
         lookup_conflict_merge_aa_set_conflict[unfolded PR_CONST_def], OF isasat_input_bounded_axioms]
@@ -1020,15 +1020,15 @@ proof -
      .
   have pre: \<open>?pre' = ?pre\<close>
     by (intro ext) (auto simp: comp_PRE_def in_br_conv list_mset_rel_def in_\<L>\<^sub>a\<^sub>l\<^sub>l_atm_of_in_atms_of_iff
-        literals_to_update_wl_empty_def option_conflict_rel_def conflict_rel_def
+        literals_to_update_wl_empty_def option_lookup_clause_rel_def lookup_clause_rel_def
         dest: literals_are_in_\<L>\<^sub>i\<^sub>n_in_\<L>\<^sub>a\<^sub>l\<^sub>l)
   have im: \<open>?im' = ?im\<close>
-    unfolding prod_hrp_comp conflict_option_assn_def
+    unfolding prod_hrp_comp option_lookup_clause_assn_def
     by (auto simp: prod_hrp_comp hrp_comp_def hr_comp_invalid)
 
   have post: \<open>?f' = ?f\<close>
     by (auto simp: list_assn_list_mset_rel_eq_list_mset_assn
-       conflict_option_assn_def)
+       option_lookup_clause_assn_def)
   show ?thesis using H unfolding PR_CONST_def pre post im .
 qed
 
@@ -1041,18 +1041,18 @@ definition (in -) is_in_lookup_option_conflict :: \<open>nat literal \<Rightarro
 
 lemma is_in_lookup_option_conflict_is_in_conflict:
   \<open>(uncurry (RETURN oo is_in_lookup_option_conflict), uncurry (RETURN oo is_in_conflict)) \<in>
-     [\<lambda>(L, C). C \<noteq> None \<and> L \<in> snd ` D\<^sub>0]\<^sub>f Id \<times>\<^sub>r option_conflict_rel \<rightarrow> \<langle>Id\<rangle>nres_rel\<close>
+     [\<lambda>(L, C). C \<noteq> None \<and> L \<in> snd ` D\<^sub>0]\<^sub>f Id \<times>\<^sub>r option_lookup_clause_rel \<rightarrow> \<langle>Id\<rangle>nres_rel\<close>
   apply (intro nres_relI frefI)
   subgoal for Lxs LC
-    using conflict_rel_atm_in_iff[of _ \<open>snd (snd (snd Lxs))\<close>]
+    using lookup_clause_rel_atm_in_iff[of _ \<open>snd (snd (snd Lxs))\<close>]
     apply (cases Lxs)
-    by (auto simp: is_in_lookup_option_conflict_def is_in_conflict_def option_conflict_rel_def)
+    by (auto simp: is_in_lookup_option_conflict_def is_in_conflict_def option_lookup_clause_rel_def)
   done
 
 sepref_definition (in -) is_in_lookup_option_conflict_code
   is \<open>uncurry (RETURN oo is_in_lookup_option_conflict)\<close>
   :: \<open>[\<lambda>(L, (b, n, xs)). atm_of L < length xs]\<^sub>a
-        unat_lit_assn\<^sup>k *\<^sub>a (bool_assn *a conflict_rel_assn)\<^sup>k \<rightarrow> bool_assn\<close>
+        unat_lit_assn\<^sup>k *\<^sub>a (bool_assn *a lookup_clause_rel_assn)\<^sup>k \<rightarrow> bool_assn\<close>
   unfolding is_in_lookup_option_conflict_def
   by sepref
 
@@ -1061,25 +1061,25 @@ lemma is_in_lookup_option_conflict_code_is_in_conflict[sepref_fr_rules]:
   \<open>(uncurry is_in_lookup_option_conflict_code,
      uncurry (RETURN oo is_in_conflict)) \<in>
     [\<lambda>(L, C). L \<in> snd ` D\<^sub>0 \<and> literals_are_in_\<L>\<^sub>i\<^sub>n (the C) \<and> C \<noteq> None]\<^sub>a
-      unat_lit_assn\<^sup>k *\<^sub>a conflict_option_assn\<^sup>k  \<rightarrow> bool_assn\<close>
+      unat_lit_assn\<^sup>k *\<^sub>a option_lookup_clause_assn\<^sup>k  \<rightarrow> bool_assn\<close>
   (is \<open>?c \<in> [?pre]\<^sub>a ?im \<rightarrow> ?f\<close>)
 proof -
   have H: \<open>?c
-    \<in> [comp_PRE (Id \<times>\<^sub>f option_conflict_rel) (\<lambda>(L, C). C \<noteq> None \<and> L \<in> snd ` D\<^sub>0)
+    \<in> [comp_PRE (Id \<times>\<^sub>f option_lookup_clause_rel) (\<lambda>(L, C). C \<noteq> None \<and> L \<in> snd ` D\<^sub>0)
           (\<lambda>_ (L, b, n, xs). atm_of L < length xs)
           (\<lambda>_. True)]\<^sub>a
-      hrp_comp (unat_lit_assn\<^sup>k *\<^sub>a (bool_assn *a conflict_rel_assn)\<^sup>k) (Id \<times>\<^sub>f option_conflict_rel)
+      hrp_comp (unat_lit_assn\<^sup>k *\<^sub>a (bool_assn *a lookup_clause_rel_assn)\<^sup>k) (Id \<times>\<^sub>f option_lookup_clause_rel)
        \<rightarrow>
       hr_comp bool_assn bool_rel\<close>
      (is \<open>_ \<in> [?pre']\<^sub>a ?im' \<rightarrow> ?f'\<close>)
     using  hfref_compI_PRE_aux[OF is_in_lookup_option_conflict_code.refine is_in_lookup_option_conflict_is_in_conflict]
     .
   have pre: \<open>?pre' x\<close> if \<open>?pre x\<close> for x
-    using that unfolding comp_PRE_def option_conflict_rel_def conflict_rel_def
-    by (auto simp: image_image in_\<L>\<^sub>a\<^sub>l\<^sub>l_atm_of_in_atms_of_iff conflict_rel_def)
+    using that unfolding comp_PRE_def option_lookup_clause_rel_def lookup_clause_rel_def
+    by (auto simp: image_image in_\<L>\<^sub>a\<^sub>l\<^sub>l_atm_of_in_atms_of_iff lookup_clause_rel_def)
   have im: \<open>?im' = ?im\<close>
     unfolding prod_hrp_comp hrp_comp_dest hrp_comp_keep
-    conflict_assn_def conflict_option_assn_def
+    lookup_clause_assn_def option_lookup_clause_assn_def
     by (auto simp: hrp_comp_def hr_comp_def)
   have f: \<open>?f' = ?f\<close>
     unfolding prod_hrp_comp hrp_comp_dest hrp_comp_keep
@@ -1136,10 +1136,10 @@ context isasat_input_ops
 begin
 
 lemma id_conflict_from_lookup:
-  \<open>(RETURN o id, conflict_from_lookup) \<in> [\<lambda>(n, xs). \<exists>D. ((n, xs), D) \<in> conflict_rel]\<^sub>f Id \<rightarrow>
-    \<langle>conflict_rel\<rangle>nres_rel\<close>
+  \<open>(RETURN o id, conflict_from_lookup) \<in> [\<lambda>(n, xs). \<exists>D. ((n, xs), D) \<in> lookup_clause_rel]\<^sub>f Id \<rightarrow>
+    \<langle>lookup_clause_rel\<rangle>nres_rel\<close>
   by (intro frefI nres_relI)
-    (auto simp: conflict_rel_def conflict_from_lookup_def RETURN_RES_refine_iff)
+    (auto simp: lookup_clause_rel_def conflict_from_lookup_def RETURN_RES_refine_iff)
 
 end
 
@@ -1148,7 +1148,7 @@ definition confl_find_next_index_spec where
      SPEC(\<lambda>j. (j \<ge> i \<and> j < length xs \<and> xs ! j \<noteq> None \<and>
         (\<forall>k. k \<ge> i \<longrightarrow> k < j \<longrightarrow> xs ! k = None))))\<close>
 
-definition confl_find_next_index :: \<open>conflict_rel \<Rightarrow> nat \<Rightarrow> nat nres\<close> where
+definition confl_find_next_index :: \<open>lookup_clause_rel \<Rightarrow> nat \<Rightarrow> nat nres\<close> where
    \<open>confl_find_next_index = (\<lambda>(n, xs) i.
       WHILE\<^sub>T\<^bsup>\<lambda>j. j < length xs \<and> (\<forall>k. k \<ge> i \<longrightarrow> k < j \<longrightarrow> xs ! k = None) \<and> j \<ge> i\<^esup>
            (\<lambda>j. xs ! j = None)
@@ -1162,7 +1162,7 @@ context isasat_input_ops
 begin
 
 lemma confl_find_next_index_confl_find_next_index_spec:
-  assumes ocr: \<open>((n, xs), D) \<in> conflict_rel\<close> and \<open>n > 0\<close> and i_xs: \<open>i < length xs\<close> and
+  assumes ocr: \<open>((n, xs), D) \<in> lookup_clause_rel\<close> and \<open>n > 0\<close> and i_xs: \<open>i < length xs\<close> and
     le_i: \<open>\<forall>k<i. xs ! k = None\<close>
   shows
     \<open>confl_find_next_index (n, xs) i \<le> confl_find_next_index_spec (n,xs) i\<close>
@@ -1171,7 +1171,7 @@ proof -
     n_D: \<open>n = size D\<close> and
     map: \<open>mset_as_position xs D\<close> and
     \<open>\<forall>L\<in>atms_of \<L>\<^sub>a\<^sub>l\<^sub>l. L < length xs\<close>
-    using ocr unfolding conflict_rel_def by auto
+    using ocr unfolding lookup_clause_rel_def by auto
   have map_empty: \<open>mset_as_position xs {#} \<longleftrightarrow> (xs = [] \<or> set xs = {None})\<close>
     by (subst mset_as_position.simps) (auto simp add: list_eq_replicate_iff)
   have ex_not_none: \<open>\<exists>j. j \<ge> i \<and> j < length xs \<and> xs ! j \<noteq> None\<close>
@@ -1271,9 +1271,9 @@ begin
 
 definition is_literal_redundant_lookup_spec where
    \<open>is_literal_redundant_lookup_spec M NU NUP D' L s =
-    SPEC(\<lambda>(s', b). b \<longrightarrow> (\<forall>D. (D', D) \<in> conflict_rel \<longrightarrow> (mset `# mset (tl NU)) + NUP \<Turnstile>pm remove1_mset L D))\<close>
+    SPEC(\<lambda>(s', b). b \<longrightarrow> (\<forall>D. (D', D) \<in> lookup_clause_rel \<longrightarrow> (mset `# mset (tl NU)) + NUP \<Turnstile>pm remove1_mset L D))\<close>
 
-definition lit_redundant_rec_wl_lookup :: \<open>(nat, nat) ann_lits \<Rightarrow> nat clauses_l \<Rightarrow> conflict_rel \<Rightarrow>
+definition lit_redundant_rec_wl_lookup :: \<open>(nat, nat) ann_lits \<Rightarrow> nat clauses_l \<Rightarrow> lookup_clause_rel \<Rightarrow>
      _ \<Rightarrow> _ \<Rightarrow>
       (_ \<times> _ \<times> bool) nres\<close>
 where
@@ -1329,7 +1329,7 @@ definition literal_redundant_wl_lookup where
 
 
 lemma lit_redundant_rec_wl_lookup_lit_redundant_rec_wl:
-  assumes D'_D: \<open>(D', D) \<in> conflict_rel\<close> and
+  assumes D'_D: \<open>(D', D) \<in> lookup_clause_rel\<close> and
     \<open>M \<Turnstile>as CNot D\<close> and
     n_d: \<open>no_dup M\<close> and
     lits: \<open>literals_are_in_\<L>\<^sub>i\<^sub>n_trail M\<close>
@@ -1344,20 +1344,20 @@ proof -
     assume ?B
     then show ?A
       using D'_D mset_as_position_nth[of \<open>snd D'\<close> D x] M that
-      unfolding conflict_rel_def
+      unfolding lookup_clause_rel_def
       by (auto simp: is_in_lookup_conflict_def split: option.splits)
   next
     assume ?A
     moreover have \<open>atm_of x < length (snd D')\<close>
       using M that D'_D
-      unfolding conflict_rel_def
+      unfolding lookup_clause_rel_def
       by (cases D') (auto simp: atms_of_\<L>\<^sub>a\<^sub>l\<^sub>l_\<A>\<^sub>i\<^sub>n in_\<L>\<^sub>a\<^sub>l\<^sub>l_atm_of_in_atms_of_iff)
     moreover have \<open>-x \<notin># D\<close>
       using \<open>M \<Turnstile>as CNot D\<close> n_d in_CNot_implies_uminus(2) no_dup_consistentD that by blast
     ultimately show ?B
       using D'_D mset_as_position_in_iff_nth[of \<open>snd D'\<close> D x] M that
         mset_as_position_in_iff_nth[of \<open>snd D'\<close> D \<open>-x\<close>]
-      unfolding conflict_rel_def
+      unfolding lookup_clause_rel_def
       by (cases x) (auto simp: is_in_lookup_conflict_def split: option.splits)
   qed
 
@@ -1397,7 +1397,7 @@ qed
 
 lemma literal_redundant_wl_lookup_literal_redundant_wl:
   assumes
-    D'_D:  \<open>(D', D) \<in> conflict_rel\<close> and
+    D'_D:  \<open>(D', D) \<in> lookup_clause_rel\<close> and
     n_d: \<open>no_dup M\<close> and
     M_D: \<open>M \<Turnstile>as CNot D\<close> and
     lits: \<open>literals_are_in_\<L>\<^sub>i\<^sub>n_trail M\<close>
@@ -1411,7 +1411,7 @@ proof -
       \<open>lit_redundant_rec_wl_lookup M NU D' cach analysis \<le> \<Down> Id
       (lit_redundant_rec_wl M' NU' D cach' analysis')\<close>
       if
-        D'_D: \<open>(D', D) \<in> conflict_rel\<close> and
+        D'_D: \<open>(D', D) \<in> lookup_clause_rel\<close> and
         M: \<open>literals_are_in_\<L>\<^sub>i\<^sub>n_trail M\<close> and
         \<open>M \<Turnstile>as CNot D\<close> and
         n_d: \<open>no_dup M\<close> and
@@ -1436,8 +1436,8 @@ proof -
 qed
 
 definition iterate_over_lookup_conflict
-  :: \<open>(nat, nat) ann_lits \<Rightarrow> nat clauses_l \<Rightarrow> conflict_rel \<Rightarrow> (nat \<Rightarrow> minimize_status) \<Rightarrow>
-       (conflict_rel \<times> (nat \<Rightarrow> minimize_status) \<times> nat conflict_highest_conflict) nres\<close>
+  :: \<open>(nat, nat) ann_lits \<Rightarrow> nat clauses_l \<Rightarrow> lookup_clause_rel \<Rightarrow> (nat \<Rightarrow> minimize_status) \<Rightarrow>
+       (lookup_clause_rel \<times> (nat \<Rightarrow> minimize_status) \<times> nat conflict_highest_conflict) nres\<close>
 where
   \<open>iterate_over_lookup_conflict  = (\<lambda>M NU (n, xs) s. do {
     (D, _, _, s, highest) \<leftarrow>
@@ -1497,7 +1497,7 @@ lemma iterate_over_lookup_conflict_iterate_over_conflict:
     NUP: \<open>NUP \<equiv> get_unit_learned S + get_unit_init_clss S\<close> and
     M': \<open>M' \<equiv> trail S'''\<close>
   assumes
-    D'_D: \<open>(D', D) \<in> conflict_rel\<close> and
+    D'_D: \<open>(D', D) \<in> lookup_clause_rel\<close> and
     M_D: \<open>M \<Turnstile>as CNot D\<close> and
     lits: \<open>literals_are_in_\<L>\<^sub>i\<^sub>n_trail M\<close> and
     struct_invs: \<open>twl_struct_invs S''\<close> and
@@ -1506,7 +1506,7 @@ lemma iterate_over_lookup_conflict_iterate_over_conflict:
     NU_P_D: \<open>NU' + NUP \<Turnstile>pm add_mset K D\<close>
   shows
     \<open>iterate_over_lookup_conflict M NU D' s' \<le>
-       \<Down> ({((D, s, L'), (D', L)). (D, D') \<in> conflict_rel \<and> L' = L})
+       \<Down> ({((D, s, L'), (D', L)). (D, D') \<in> lookup_clause_rel \<and> L' = L})
            (iterate_over_conflict K M NU' NUP D)\<close>
     (is \<open>_ \<le> \<Down> ?R _\<close>)
 proof -
@@ -1546,9 +1546,9 @@ proof -
   define R where
     \<open>R = {(((n, xs), m, i, cach :: nat \<Rightarrow> minimize_status, highest':: nat conflict_highest_conflict),
             (F :: nat clause, E :: nat clause, highest:: nat conflict_highest_conflict)).
-            ((n, xs), F) \<in> conflict_rel \<and>
+            ((n, xs), F) \<in> lookup_clause_rel \<and>
             i \<le> length xs \<and>
-            ((m, replicate i None @ drop i xs), E) \<in> conflict_rel \<and>
+            ((m, replicate i None @ drop i xs), E) \<in> lookup_clause_rel \<and>
             n \<ge> m \<and>
             F \<subseteq># D \<and>
             E \<subseteq># F \<and>
@@ -1566,8 +1566,8 @@ proof -
       \<open>iterate_over_conflict_inv M D s\<close>
     for s' s
    proof -
-     have \<open>((a, b), x) \<in> conflict_rel \<Longrightarrow> a \<le> length b\<close> for a b x
-       by (auto simp: conflict_rel_def dest!: mset_as_position_length_not_None)
+     have \<open>((a, b), x) \<in> lookup_clause_rel \<Longrightarrow> a \<le> length b\<close> for a b x
+       by (auto simp: lookup_clause_rel_def dest!: mset_as_position_length_not_None)
     then show ?thesis
       using that unfolding iterate_over_lookup_conflict_inv_def by (auto simp: R_def)
   qed
@@ -1587,7 +1587,7 @@ proof -
   proof -
     show ?thesis
       using st'_st unfolding st
-      by (cases D') (auto simp: R_def conflict_rel_def)
+      by (cases D') (auto simp: R_def lookup_clause_rel_def)
   qed
   have confl_find_next_index_spec_le:
     \<open>confl_find_next_index_spec (x1d, x2b) x1e
@@ -1608,7 +1608,7 @@ proof -
     for x x' x1 x1a x1b x1c x2b x2c x1d x2d x1e x2e st2 st3
   proof -
     have map: \<open>mset_as_position (replicate x1e None @ drop x1e x2b) x1a\<close>
-      using R unfolding st R_def conflict_rel_def
+      using R unfolding st R_def lookup_clause_rel_def
       by auto
     show ?thesis
       unfolding confl_find_next_index_spec_def st
@@ -1653,9 +1653,9 @@ proof -
   proof -
     let ?L = \<open>(if the (xs ! a) then Pos a else Neg a)\<close>
     have
-      cr: \<open>((n, xs), E) \<in> conflict_rel\<close> and
+      cr: \<open>((n, xs), E) \<in> lookup_clause_rel\<close> and
       \<open>x1e \<le> length xs\<close> and
-      \<open>((x1d, replicate x1e None @ drop x1e xs), x1a) \<in> conflict_rel\<close> and
+      \<open>((x1d, replicate x1e None @ drop x1e xs), x1a) \<in> lookup_clause_rel\<close> and
       \<open>x1d \<le> n\<close> and
       \<open>E \<subseteq># D\<close> and
       \<open>x1a \<subseteq># E\<close> and
@@ -1746,9 +1746,9 @@ proof -
     have L: \<open>L = (if the (xs ! m'') then Pos m'' else Neg m'')\<close>
       using xa_xb by auto
     have
-      x1c_x1[simp]: \<open>((n, xs), D') \<in> conflict_rel\<close> and
+      x1c_x1[simp]: \<open>((n, xs), D') \<in> lookup_clause_rel\<close> and
       [simp]: \<open>i \<le> length xs\<close> and
-      x1d_x1a: \<open>((m, replicate i None @ drop i xs), D'') \<in> conflict_rel\<close> and
+      x1d_x1a: \<open>((m, replicate i None @ drop i xs), D'') \<in> lookup_clause_rel\<close> and
       x1d_x1c: \<open>m \<le> n\<close> and
       incls: \<open>D' \<subseteq># D\<close> \<open>D'' \<subseteq># D'\<close> and
       [simp]: \<open>highest' = highest\<close> and
@@ -1787,7 +1787,7 @@ proof -
       x1d: \<open>m = size D''\<close> and
       map: \<open>mset_as_position (replicate i None @ drop i xs) D''\<close> and
       L_all_x2b: \<open>\<forall>L\<in>atms_of \<L>\<^sub>a\<^sub>l\<^sub>l. L < length xs\<close>
-      using x1d_x1a unfolding conflict_rel_def by auto
+      using x1d_x1a unfolding lookup_clause_rel_def by auto
 
     have 4: \<open>(replicate m'' None @ drop m'' xs)[m'' := None] =
         replicate (Suc m'') None @ drop (Suc m'') xs\<close>
@@ -1808,9 +1808,9 @@ proof -
 
     then have map':
       \<open>((m - Suc 0, replicate (Suc m'') None @ drop (Suc m'') xs), remove1_mset L D'')
-        \<in> conflict_rel\<close>
+        \<in> lookup_clause_rel\<close>
       using xb_x1a x1d L_all_x2b
-      by (auto simp: size_remove1_mset_If conflict_rel_def simp del: replicate_Suc)
+      by (auto simp: size_remove1_mset_If lookup_clause_rel_def simp del: replicate_Suc)
     show H: ?loop_keep if \<open>\<not>red\<close>
       using xa_xb x1d_x1c map' incls cach that keep unfolding R_def L[symmetric] st
       by (auto intro: subset_mset.order.trans diff_subset_eq_self)
@@ -1819,7 +1819,7 @@ proof -
       \<open>n = size D'\<close> and
       map: \<open>mset_as_position xs D'\<close> and
       \<open>\<forall>L\<in>atms_of \<L>\<^sub>a\<^sub>l\<^sub>l. L < length xs\<close>
-      using x1c_x1 unfolding conflict_rel_def by auto
+      using x1c_x1 unfolding lookup_clause_rel_def by auto
     have [simp]: \<open>D' - {#Pos m'', Neg m''#} = remove1_mset L D'\<close> \<open>L \<in># D'\<close>
       using mset_as_position_in_iff_nth[OF map, of \<open>Pos m''\<close>]
         mset_as_position_in_iff_nth[OF map, of \<open>Neg m''\<close>] xa_le_x2b no_none
@@ -1829,8 +1829,8 @@ proof -
       using mset_as_position_remove[OF map, of \<open>m''\<close>] xa_le_x2b
       by (auto simp del: replicate_Suc simp: 3 4)
 
-    then have \<open>((n - Suc 0, xs[m'' := None]), remove1_mset L D') \<in> conflict_rel\<close>
-      using x1c_x1 unfolding conflict_rel_def
+    then have \<open>((n - Suc 0, xs[m'' := None]), remove1_mset L D') \<in> lookup_clause_rel\<close>
+      using x1c_x1 unfolding lookup_clause_rel_def
       by (auto simp: size_remove1_mset_If)
     moreover have  \<open>m - Suc 0 \<le> n - Suc 0\<close>
       using diff_le_mono x1d_x1c by blast
@@ -1971,7 +1971,7 @@ sepref_thm lit_redundant_rec_wl_lookup_code
          literals_are_in_\<L>\<^sub>i\<^sub>n_trail M \<and>
          (\<forall>a \<in> lits_of_l M. atm_of a < length (snd D))
       ]\<^sub>a
-      trail_assn\<^sup>k *\<^sub>a clauses_ll_assn\<^sup>k *\<^sub>a conflict_rel_assn\<^sup>k *\<^sub>a
+      trail_assn\<^sup>k *\<^sub>a clauses_ll_assn\<^sup>k *\<^sub>a lookup_clause_rel_assn\<^sup>k *\<^sub>a
         cach_refinement_assn\<^sup>d *\<^sub>a analyse_refinement_assn\<^sup>d \<rightarrow>
       cach_refinement_assn *a analyse_refinement_assn *a bool_assn\<close>
   supply [[goals_limit = 1]] neq_Nil_revE[elim] image_image[simp]
@@ -2090,7 +2090,7 @@ lemma
     NUP: \<open>NUP \<equiv> get_unit_learned S + get_unit_init_clss S\<close> and
     M': \<open>M' \<equiv> trail S'''\<close>
   assumes
-    D'_D: \<open>(D', D) \<in> conflict_rel\<close> and
+    D'_D: \<open>(D', D) \<in> lookup_clause_rel\<close> and
     M_D: \<open>M \<Turnstile>as CNot D\<close> and
     lits: \<open>literals_are_in_\<L>\<^sub>i\<^sub>n_trail M\<close> and
     struct_invs: \<open>twl_struct_invs S''\<close> and
@@ -2100,11 +2100,11 @@ lemma
     confl: \<open>get_conflict_wl S \<noteq> None\<close>
   shows
     \<open>iterate_over_lookup_conflict M NU D' s' \<le>
-       \<Down> ({((D, s, L'), (D', L)). (D, D') \<in> conflict_rel \<and> L' = L})
+       \<Down> ({((D, s, L'), (D', L)). (D, D') \<in> lookup_clause_rel \<and> L' = L})
             (SPEC (\<lambda>(D', highest). D' \<subseteq># D \<and> NU' + NUP \<Turnstile>pm add_mset K D' \<and> highest_lit M D' highest))\<close>
 proof -
   have dist: \<open>distinct_mset D\<close>
-    using D'_D unfolding conflict_rel_def
+    using D'_D unfolding lookup_clause_rel_def
     by (auto dest: mset_as_position_distinct_mset)
   show ?thesis
     apply (rule order.trans)
@@ -2118,7 +2118,7 @@ qed
 end
 term \<open>(uncurry extract_shorter_conflict_list_removed,
           uncurry (RETURN oo extract_shorter_conflict_l_trivial)) \<in>
-      [\<lambda>(M', D). literals_are_in_\<L>\<^sub>i\<^sub>n (the D) \<and> D \<noteq> None \<and> M = M']\<^sub>f Id \<times>\<^sub>f option_conflict_rel \<rightarrow>
-         \<langle>{((D, L), C). (D, C) \<in> option_conflict_rel \<and> C \<noteq> None \<and> highest_lit M (the C) L \<and>
+      [\<lambda>(M', D). literals_are_in_\<L>\<^sub>i\<^sub>n (the D) \<and> D \<noteq> None \<and> M = M']\<^sub>f Id \<times>\<^sub>f option_lookup_clause_rel \<rightarrow>
+         \<langle>{((D, L), C). (D, C) \<in> option_lookup_clause_rel \<and> C \<noteq> None \<and> highest_lit M (the C) L \<and>
            (\<forall>L\<in>atms_of \<L>\<^sub>a\<^sub>l\<^sub>l. L < length (snd (snd D)))}\<rangle> nres_rel\<close>
 end
